Everything compiles up unto Reify.v

Java/src/Java/Func/JavaFunc.v
@@ -1,29 +1,36 @@
-Require Import Charge.Open.Subst.
-Require Import Charge.Open.Open.
-Require Import Charge.Open.Stack.
-Require Import Charge.Logics.BILogic.
-Require Import Charge.ModularFunc.ILogicFunc.
-Require Import Charge.ModularFunc.BILogicFunc.
-Require Import Charge.ModularFunc.LaterFunc.
-Require Import Charge.ModularFunc.BaseFunc.
-Require Import Charge.ModularFunc.ListFunc.
-Require Import Charge.ModularFunc.OpenFunc.
-Require Import Charge.ModularFunc.EmbedFunc.
+Require Import ChargeCore.Open.Subst.
+Require Import ChargeCore.Open.Open.
+Require Import ChargeCore.Open.Stack.
+Require Import ChargeCore.Logics.BILogic.
+Require Import Charge.Views.ILogicView.
+Require Import Charge.Views.BILogicView.
+Require Import Charge.Views.SubstView.
+Require Import Charge.Views.EmbedView.
 
 Require Import ExtLib.Core.RelDec.
 Require Import ExtLib.Data.Fun.
 Require Import ExtLib.Data.String.
 Require Import ExtLib.Data.Sum.
+Require Import ExtLib.Data.Positive.
+Require Import ExtLib.Data.SumN.
+Require Import ExtLib.Data.Map.FMapPositive.
 Require Import ExtLib.Tactics.Consider.
 
 Require Import MirrorCore.TypesI.
 Require Import MirrorCore.SymI.
 Require Import MirrorCore.Lemma.
 Require Import MirrorCore.Lambda.Expr.
+Require Import MirrorCore.Views.FuncView.
 Require Import MirrorCore.syms.SymEnv.
 Require Import MirrorCore.syms.SymSum.
+Require Import MirrorCore.syms.SymOneOf.
 Require Import MirrorCore.Subst.FMapSubst.
-Set Printing Universes.
+Require Import MirrorCore.Views.ListView.
+Require Import MirrorCore.Views.ProdView.
+Require Import MirrorCore.Views.ApplicativeView.
+Require Import MirrorCore.Views.NatView.
+Require Import MirrorCore.Views.StringView.
+
 Require Import Java.Logic.AssertionLogic.
 Require Import Java.Logic.SpecLogic.
 Require Import Java.Language.Lang.
@@ -37,232 +44,293 @@ Require Import Coq.Bool.Bool.
 Set Implicit Arguments.
 Set Strict Implicit.
 
-	Inductive java_func :=
+Inductive java_func :=
+| pProg (p : Program)
+| pMethod (m : Method)
+| pVal (v : val)
+| pCmd (c : cmd)
+| pExpr (e : dexpr)
+| pFields (f : list string)
+          
+| pMethodSpec
+| pProgEq
+| pTriple
+| pTypeOf
+| pFieldLookup
+| pMethodLookup
+    
+| pPointsto
+| pNull
+    
+| pMethodBody
+| pMethodArgs
+| pMethodRet
+    
+    
+| pPlus
+| pMinus
+| pTimes
+| pAnd
+| pOr
+| pNot
+| pLt
+| pValEq.
 
-	| pMethodSpec
-	| pProgEq
-	| pTriple
-	| pTypeOf
-	| pFieldLookup
-	| pMethodLookup
-	
-	| pPointsto
-	| pNull
-	
-	| pMethodBody
-	| pMethodArgs
-	| pMethodRet
-	
-	
-	| pPlus
-	| pMinus
-	| pTimes
-	| pAnd
-	| pOr
-	| pNot
-	| pLt
-	| pValEq.
+Fixpoint beq_list {A} (f : A -> A -> bool) (xs ys : list A) :=
+  match xs, ys with
+  | nil, nil => true
+  | x::xs, y :: ys => andb (f x y) (beq_list f xs ys)
+  | _, _ => false
+  end.
 
-	Fixpoint beq_list {A} (f : A -> A -> bool) (xs ys : list A) :=
-		match xs, ys with
-			| nil, nil => true
-			| x::xs, y :: ys => andb (f x y) (beq_list f xs ys)
-			| _, _ => false
-		end.
-
-	Definition typeof_java_func bf :=
-		match bf with
-		    | pMethodSpec => Some (tyArr tyString (tyArr tyString (tyArr tyVarList
-		    	 (tyArr tyString (tyArr tySasn (tyArr tySasn tySpec))))))
-		    | pProgEq => Some (tyArr tyProg tySpec)
-		    | pTriple => Some (tyArr tySasn (tyArr tySasn (tyArr tyCmd tySpec)))
+Definition typeof_java_func bf :=
+  match bf with
+  | pProg _ => Some tyProg
+  | pCmd _ => Some tyCmd
+  | pMethod _ => Some tyMethod
+  | pVal _ => Some tyVal
+  | pExpr _ => Some tyDExpr
+  | pFields _ => Some (tyList tyString)
+		      
+  | pMethodSpec => Some (tyArr tyString (tyArr tyString (tyArr tyVarList
+		    	                                       (tyArr tyString (tyArr tySasn (tyArr tySasn tySpec))))))
+  | pProgEq => Some (tyArr tyProg tySpec)
+  | pTriple => Some (tyArr tySasn (tyArr tySasn (tyArr tyCmd tySpec)))
 		    
-		    | pTypeOf => Some (tyArr tyString (tyArr tyVal tyProp))
+  | pTypeOf => Some (tyArr tyString (tyArr tyVal tyProp))
 		    
-		    | pFieldLookup => Some (tyArr tyProg (tyArr tyString (tyArr tyFields tyProp)))
-		    | pMethodLookup => Some (tyArr tyProg (tyArr tyString (tyArr tyString (tyArr tyMethod tyProp))))
+  | pFieldLookup => Some (tyArr tyProg (tyArr tyString (tyArr tyFields tyProp)))
+  | pMethodLookup => Some (tyArr tyProg (tyArr tyString (tyArr tyString (tyArr tyMethod tyProp))))
 		    
-		    | pPointsto => Some (tyArr tyVal (tyArr tyString (tyArr tyVal tyAsn)))
-		    | pNull => Some tyVal
-		    
-		    | pMethodBody => Some (tyArr tyMethod tyCmd)
-		    | pMethodArgs => Some (tyArr tyMethod (tyList tyString))
-		    | pMethodRet => Some (tyArr tyMethod tyDExpr)
-		    
-		    | pPlus => Some (tyArr tyVal (tyArr tyVal tyVal))
-		    | pMinus => Some (tyArr tyVal (tyArr tyVal tyVal))
-		    | pTimes => Some (tyArr tyVal (tyArr tyVal tyVal))
-		    | pAnd => Some (tyArr tyVal (tyArr tyVal tyVal))
-		    | pOr => Some (tyArr tyVal (tyArr tyVal tyVal))
-		    | pNot => Some (tyArr tyVal tyVal)
-		    | pLt => Some (tyArr tyVal (tyArr tyVal tyVal))
-		    | pValEq => Some (tyArr tyVal (tyArr tyVal tyVal))
-		end.
+  | pPointsto => Some (tyArr tyVal (tyArr tyString (tyArr tyVal tyAsn)))
+  | pNull => Some tyVal
+		  
+  | pMethodBody => Some (tyArr tyMethod tyCmd)
+  | pMethodArgs => Some (tyArr tyMethod (tyList tyString))
+  | pMethodRet => Some (tyArr tyMethod tyDExpr)
+		       
+  | pPlus => Some (tyArr tyVal (tyArr tyVal tyVal))
+  | pMinus => Some (tyArr tyVal (tyArr tyVal tyVal))
+  | pTimes => Some (tyArr tyVal (tyArr tyVal tyVal))
+  | pAnd => Some (tyArr tyVal (tyArr tyVal tyVal))
+  | pOr => Some (tyArr tyVal (tyArr tyVal tyVal))
+  | pNot => Some (tyArr tyVal tyVal)
+  | pLt => Some (tyArr tyVal (tyArr tyVal tyVal))
+  | pValEq => Some (tyArr tyVal (tyArr tyVal tyVal))
+  end.
 
-	Definition java_func_eq (a b : java_func) : option bool :=
-	  match a , b with
-	    | pMethodSpec, pMethodSpec => Some true
-	    | pProgEq, pProgEq => Some true
-		| pTriple, pTriple => Some true
-	
-	    | pTypeOf, pTypeOf => Some true
-	
-	    | pPointsto, pPointsto => Some true
-	    | pFieldLookup, pFieldLookup => Some true
-	    | pMethodLookup, pMethodLookup => Some true
-	    
-	    | pMethodBody, pMethodBody => Some true
-	    | pMethodArgs, pMethodArgs => Some true
-	    | pMethodRet, pMethodRet => Some true
-	
-	    | pNull, pNull => Some true
-	    | pPlus, pPlus => Some true
-	    | pMinus, pMinus => Some true
-	    | pTimes, pTimes => Some true
-	    | pAnd, pAnd => Some true
-	    | pOr, pOr => Some true
-	    | pNot, pNot => Some true
-	    | pLt, pLt => Some true
-	    | pValEq, pValEq => Some true
-	    | _, _ => None
-	  end.
+Definition java_func_eq (a b : java_func) : option bool :=
+  match a , b with
+  | pProg p1, pProg p2 => Some (p1 ?[ eq ] p2)
+  | pMethod m1, pMethod m2 => Some (m1 ?[ eq ] m2)
+  | pVal v1, pVal v2 => Some (v1 ?[ eq ] v2)
+  | pExpr e1, pExpr e2 => Some (e1 ?[ eq ] e2)
+  | pFields f1, pFields f2 => Some (f1 ?[ eq ] f2)
+  | pCmd c1, pCmd c2 => Some (c1 ?[ eq ]c2)
+	                     
+  | pMethodSpec, pMethodSpec => Some true
+  | pProgEq, pProgEq => Some true
+  | pTriple, pTriple => Some true
+	                     
+  | pTypeOf, pTypeOf => Some true
+	                     
+  | pPointsto, pPointsto => Some true
+  | pFieldLookup, pFieldLookup => Some true
+  | pMethodLookup, pMethodLookup => Some true
+	                                 
+  | pMethodBody, pMethodBody => Some true
+  | pMethodArgs, pMethodArgs => Some true
+  | pMethodRet, pMethodRet => Some true
+	                           
+  | pNull, pNull => Some true
+  | pPlus, pPlus => Some true
+  | pMinus, pMinus => Some true
+  | pTimes, pTimes => Some true
+  | pAnd, pAnd => Some true
+  | pOr, pOr => Some true
+  | pNot, pNot => Some true
+  | pLt, pLt => Some true
+  | pValEq, pValEq => Some true
+  | _, _ => None
+  end.
 
-    Global Instance RelDec_java_func : RelDec (@eq java_func) := {
-      rel_dec a b := match java_func_eq a b with 
-    	  		       | Some b => b 
-    		 	       | None => false 
-    			     end
-    }.
+Global Instance RelDec_java_func : RelDec (@eq java_func) := 
+  {
+    rel_dec a b := match java_func_eq a b with 
+    	  	   | Some b => b 
+    		   | None => false 
+    		   end
+  }.
 
-    Global Instance RelDec_Correct_java_func : RelDec_Correct RelDec_java_func.
-    Proof.
-      constructor.
-      destruct x; destruct y; simpl;
-      try solve [ try rewrite Bool.andb_true_iff ;
-                  repeat rewrite rel_dec_correct; intuition congruence ].                  	
-    Qed.
+Global Instance RelDec_Correct_java_func : RelDec_Correct RelDec_java_func.
+Proof.
+  constructor.
+  destruct x; destruct y; simpl;
+  try solve [ try rewrite Bool.andb_true_iff ;
+              repeat rewrite rel_dec_correct; intuition congruence ].                  	
+Qed.
 (*
 Definition set_fold_fun (x : String.string) (f : field) (P : sasn) :=
 	(liftn pointsto) (x/V) `f `null ** P.
 *)
-  	 Definition java_func_symD bf :=
-		match bf as bf return match typeof_java_func bf with
-								| Some t => typD t
-								| None => unit
-							  end with
-              | pMethodSpec => method_spec
-              | pProgEq => prog_eq
-              | pTriple => triple
-              
-              | pTypeOf => typeof
-                            
-              | pFieldLookup => field_lookup
-              | pMethodLookup => method_lookup
-              
-              | pPointsto => pointsto
-              
-              | pNull => null
-              
-              | pMethodBody => m_body
-              | pMethodArgs => m_params
-              | pMethodRet => m_ret
-              
-              | pPlus => eplus
-              | pMinus => eminus
-              | pTimes => etimes
-              | pAnd => eand
-              | pOr => eor
-              | pNot => enot
-              | pLt => elt
-              | pValEq => eeq
-	end.
+Definition java_func_symD bf :=
+  match bf as bf return match typeof_java_func bf with
+			| Some t => typD t
+			| None => unit
+			end with
+    
+  | pProg p => p
+  | pMethod m => m
+  | pVal v => v
+  | pExpr e => e
+  | pFields f => f
+  | pCmd c => c
+  | pMethodSpec => method_spec
+  | pProgEq => prog_eq
+  | pTriple => triple
+                 
+  | pTypeOf => typeof
+                 
+  | pFieldLookup => field_lookup
+  | pMethodLookup => method_lookup
+                       
+  | pPointsto => pointsto
+                   
+  | pNull => null
+               
+  | pMethodBody => m_body
+  | pMethodArgs => m_params
+  | pMethodRet => m_ret
+                    
+  | pPlus => eplus
+  | pMinus => eminus
+  | pTimes => etimes
+  | pAnd => eand
+  | pOr => eor
+  | pNot => enot
+  | pLt => elt
+  | pValEq => eeq
+  end.
 
-	Global Instance RSym_JavaFunc : SymI.RSym java_func := {
-	  typeof_sym := typeof_java_func;
-	  symD := java_func_symD;
-	  sym_eqb := java_func_eq
-	}.
+Global Instance RSym_JavaFunc : SymI.RSym java_func := 
+  {
+    typeof_sym := typeof_java_func;
+    symD := java_func_symD;
+    sym_eqb := java_func_eq
+  }.
 
-	Global Instance RSymOk_JavaFunc : SymI.RSymOk RSym_JavaFunc.
-	Proof.
-		split; intros.
-		destruct a, b; simpl; try apply I; try reflexivity.
-	Qed.		
+Global Instance RSymOk_JavaFunc : SymI.RSymOk RSym_JavaFunc.
+Proof.
+  split; intros.
+  destruct a, b; simpl; try apply I; try reflexivity.
+  consider (p ?[ eq ] p0); intros; subst; intuition congruence.
+  consider (m ?[ eq ] m0); intros; subst; intuition congruence.
+  consider (v ?[ eq ] v0); intros; subst; intuition congruence.
+  consider (c ?[ eq ] c0); intros; subst; intuition congruence.
+  consider (e ?[ eq ] e0); intros; subst; intuition congruence.
+  consider (f ?[ eq ] f0); intros; subst; intuition congruence.
+Qed.	
 
-Global Instance RelDec_bf_false : RelDec (@eq (@base_func typ RType_typ)) := {
-  rel_dec := fun a b => match (base_func_eq a b) with | Some t => t | None => false end
-}.
+Fixpoint list_to_pmap_aux {T : Type} (lst : list T) (p : positive) : pmap T :=
+  match lst with
+    | nil => Empty
+    | x :: xs => pmap_insert p x (list_to_pmap_aux xs (p + 1))
+  end.
+  
+Definition list_to_pmap {T : Type} (lst : list Type) := list_to_pmap_aux lst 1.
 
-Definition func := (SymEnv.func + @ilfunc typ + @bilfunc typ + 
-                    @base_func typ RType_typ + @list_func typ + @open_func typ _ _+ 
-                    @embed_func typ + @later_func typ + java_func)%type.
+Definition func_map : pmap Type :=
+	list_to_pmap (T := Type) 
+	  (java_func::SymEnv.func::@ilfunc typ::@bilfunc typ::@list_func typ::
+	   @subst_func typ::@embed_func typ::(natFunc:Type)::(stringFunc:Type)::
+           @prod_func typ::@ap_func typ::nil).
 
+Definition func := OneOf func_map.
 
-Notation pProg P := (Inj (inl (inl (inl (inl (inl (inr (pConst tyProg P)))))))).
-Notation pMethod M := (Inj (inl (inl (inl (inl (inl (inr (pConst tyMethod M)))))))).
+Global Instance ILogicView_func : FuncView func (@ilfunc typ) :=
+  FuncViewPMap 3func_map eq_refl.
+Global Instance BILogicView_func : FuncView func (@bilfunc typ) :=
+  FuncViewPMap 4 func_map eq_refl.
+Global Instance ListView_func : FuncView func (@list_func typ) :=
+  FuncViewPMap 5 func_map eq_refl.
+Global Instance SubstView_func : FuncView func (@subst_func typ) :=
+  FuncViewPMap 6 func_map eq_refl.
+Global Instance EmbedView_func : FuncView func (@embed_func typ) :=
+  FuncViewPMap 7 func_map eq_refl.
+Global Instance NatView_func : FuncView func natFunc :=
+  FuncViewPMap 8 func_map eq_refl.
+Global Instance StringView_func : FuncView func stringFunc :=
+  FuncViewPMap 9 func_map eq_refl.
+Global Instance ProdView_func : FuncView func (@prod_func typ) :=
+  FuncViewPMap 10 func_map eq_refl.
+Global Instance ApplicativeView_func : FuncView func (@ap_func typ) :=
+  FuncViewPMap 11 func_map eq_refl.
 
 Section MakeJavaFunc.
 
-	Definition mkVal v : expr typ func := Inj (inl (inl (inl (inl (inl (inr (pConst tyVal v))))))).
-	Definition mkProg P : expr typ func := pProg P.
-	Definition mkMethod M : expr typ func := pMethod M.
-	Definition mkCmd c : expr typ func := Inj (inl (inl (inl (inl (inl (inr (pConst tyCmd c))))))).
-	Definition mkDExpr e : expr typ func := Inj (inl (inl (inl (inl (inl (inr (pConst tyDExpr e))))))).
-	Definition mkFields fs : expr typ func := Inj (inl (inl (inl (inl (inl (inr (pConst (tyList tyString) fs))))))).
+  Definition mkJavaFunc (f : java_func) : expr typ func := 
+    Inj (Into (ts := func_map) f 1 eq_refl).
 
-	Definition fMethodSpec : expr typ func := Inj (inr pMethodSpec).
-	Definition fProgEq : expr typ func := Inj (inr pProgEq).
-	Definition fTriple : expr typ func := Inj (inr pTriple).
-	Definition fTypeOf : expr typ func := Inj (inr pTypeOf).
-	Definition fFieldLookup : expr typ func := Inj (inr pFieldLookup).
-	Definition fMethodLookup : expr typ func := Inj (inr pMethodLookup).
-	Definition fPointsto : expr typ func := Inj (inr pPointsto).
-	Definition mkNull : expr typ func := Inj (inr pNull).
+  Definition mkVal v : expr typ func := mkJavaFunc (pVal v).
+  Definition mkProg P : expr typ func := mkJavaFunc (pProg P).
+  Definition mkMethod M : expr typ func := mkJavaFunc (pMethod M).
+  Definition mkCmd c : expr typ func := mkJavaFunc (pCmd c).
+  Definition mkDExpr e : expr typ func := mkJavaFunc (pExpr e).
+  Definition mkFields f : expr typ func := mkJavaFunc (pFields f).
+  
+  Definition fMethodSpec : expr typ func := mkJavaFunc pMethodSpec.
+  Definition fProgEq : expr typ func := mkJavaFunc pProgEq.
+  Definition fTriple : expr typ func := mkJavaFunc pTriple.
+  Definition fTypeOf : expr typ func := mkJavaFunc pTypeOf.
+  Definition fFieldLookup : expr typ func := mkJavaFunc pFieldLookup.
+  Definition fMethodLookup : expr typ func := mkJavaFunc pMethodLookup.
+  Definition fPointsto : expr typ func := mkJavaFunc pPointsto.
+  Definition mkNull : expr typ func := mkJavaFunc pNull.
+  
+  Definition fMethodBody : expr typ func := mkJavaFunc pMethodBody.
+  Definition fMethodArgs : expr typ func := mkJavaFunc pMethodArgs.
+  Definition fMethodRet : expr typ func := mkJavaFunc pMethodRet.	
+  
+  Definition fPlus : expr typ func := mkJavaFunc pPlus.
+  Definition fMinus : expr typ func := mkJavaFunc pMinus.
+  Definition fTimes : expr typ func := mkJavaFunc pTimes.
+  Definition fAnd : expr typ func := mkJavaFunc pAnd.
+  Definition fOr : expr typ func := mkJavaFunc pOr.
+  Definition fNot : expr typ func := mkJavaFunc pNot.
+  Definition fLt : expr typ func := mkJavaFunc pLt.
+  Definition fValEq : expr typ func := mkJavaFunc pValEq.
 
-	Definition fMethodBody : expr typ func := Inj (inr pMethodBody).
-	Definition fMethodArgs : expr typ func := Inj (inr pMethodArgs).
-	Definition fMethodRet : expr typ func := Inj (inr pMethodRet).	
-	
-	Definition fPlus : expr typ func := Inj (inr pPlus).
-	Definition fMinus : expr typ func := Inj (inr pMinus).
-	Definition fTimes : expr typ func := Inj (inr pTimes).
-	Definition fAnd : expr typ func := Inj (inr pAnd).
-	Definition fOr : expr typ func := Inj (inr pOr).
-	Definition fNot : expr typ func := Inj (inr pNot).
-	Definition fLt : expr typ func := Inj (inr pLt).
-	Definition fValEq : expr typ func := Inj (inr pValEq).
+  Definition mkTriple P c Q : expr typ func := App (App (App fTriple P) Q) c.
+  Definition mkFieldLookup P C f : expr typ func := App (App (App fFieldLookup P) C) f.
+  Definition mkTypeOf C x : expr typ func := App (App fTypeOf C) x.
+  Definition mkProgEq P := App fProgEq P.
+  
+  Definition mkMethodBody (M : Method) : expr typ func := App fMethodBody (mkMethod M).
+  Definition mkMethodArgs (M : Method) : expr typ func := App fMethodArgs (mkMethod M).
+  Definition mkMethodRet (M : Method) : expr typ func := App fMethodRet (mkMethod M).
 
-	Definition mkTriple P c Q : expr typ func := App (App (App fTriple P) Q) c.
-	Definition mkFieldLookup P C f : expr typ func := App (App (App fFieldLookup P) C) f.
-	Definition mkTypeOf C x : expr typ func := App (App fTypeOf C) x.
-	Definition mkProgEq P := App fProgEq P.
 	
-	Definition mkMethodBody (M : Method) : expr typ func := App fMethodBody (mkMethod M).
-	Definition mkMethodArgs (M : Method) : expr typ func := App fMethodArgs (mkMethod M).
-	Definition mkMethodRet (M : Method) : expr typ func := App fMethodRet (mkMethod M).
-	
-	Definition mkExprList es :=
-		(fold_right (fun (e : dexpr) (acc : expr typ func) => 
-			mkCons tyExpr (mkDExpr e) acc) (mkNil tyExpr) es).
-	
-	Fixpoint evalDExpr (e : dexpr) : expr typ func :=
-		match e with
-			| E_val v => mkConst tyVal (mkVal v)
-			| E_var x => App (fStackGet (func := expr typ func)) (mkString (func := func) x)
-			| E_plus e1 e2 => mkAps fPlus ((evalDExpr e2, tyVal)::(evalDExpr e1, tyVal)::nil) tyVal
-			| E_minus e1 e2 => mkAps fMinus ((evalDExpr e2, tyVal)::(evalDExpr e1, tyVal)::nil) tyVal
-			| E_times e1 e2 => mkAps fTimes ((evalDExpr e2, tyVal)::(evalDExpr e1, tyVal)::nil) tyVal
-			| E_and e1 e2 => mkAps fAnd ((evalDExpr e2, tyVal)::(evalDExpr e1, tyVal)::nil) tyVal
-			| E_or e1 e2 => mkAps fOr ((evalDExpr e2, tyVal)::(evalDExpr e1, tyVal)::nil) tyVal
-			| E_not e => mkAps fNot ((evalDExpr e, tyVal)::nil) tyVal
-			| E_lt e1 e2 => mkAps fLt ((evalDExpr e2, tyVal)::(evalDExpr e1, tyVal)::nil) tyVal
-			| E_eq e1 e2 => mkAps fValEq ((evalDExpr e2, tyVal)::(evalDExpr e1, tyVal)::nil) tyVal
-		end.
+  Definition mkExprList es :=
+    (fold_right (fun (e : dexpr) (acc : expr typ func) => 
+		   mkCons tyExpr (mkDExpr e) acc) (mkNil tyExpr) es).
 
+Check @fStackGet.
+
+Fixpoint evalDExpr (e : dexpr) : expr typ func :=
+    match e with
+    | E_val v => mkVal v
+    | E_var x => App (Inj fStackGet) (mkString x)
+    | E_plus e1 e2 => mkAps fPlus ((evalDExpr e2, tyVal)::(evalDExpr e1, tyVal)::nil) tyVal
+    | E_minus e1 e2 => mkAps fMinus ((evalDExpr e2, tyVal)::(evalDExpr e1, tyVal)::nil) tyVal
+    | E_times e1 e2 => mkAps fTimes ((evalDExpr e2, tyVal)::(evalDExpr e1, tyVal)::nil) tyVal
+    | E_and e1 e2 => mkAps fAnd ((evalDExpr e2, tyVal)::(evalDExpr e1, tyVal)::nil) tyVal
+    | E_or e1 e2 => mkAps fOr ((evalDExpr e2, tyVal)::(evalDExpr e1, tyVal)::nil) tyVal
+    | E_not e => mkAps fNot ((evalDExpr e, tyVal)::nil) tyVal
+    | E_lt e1 e2 => mkAps fLt ((evalDExpr e2, tyVal)::(evalDExpr e1, tyVal)::nil) tyVal
+    | E_eq e1 e2 => mkAps fValEq ((evalDExpr e2, tyVal)::(evalDExpr e1, tyVal)::nil) tyVal
+    end.
 
 End MakeJavaFunc.
-
-Require Import Java.Examples.ListModel.
 
 
 Class Environment := { java_env :> @SymEnv.functions typ _}.
@@ -286,28 +354,89 @@ Check RSym.
 	  RSym_bilfunc bilops.
   Global Instance RSym_embed_func : RSym (@embed_func typ) :=
 	  RSym_embed_func eops.
-  Global Instance RSym_later_func : RSym (@later_func typ) :=
-	  RSym_later_func _ lops.
+(*  Global Instance RSym_later_func : RSym (@later_func typ) :=
+	  RSym_later_func _ lops.*)
 (*
   Global Instance RelDec_func : RelDec (@eq func).
   repeat apply RelDec_eq_pair; try apply _.
   apply _.
 *)
-  Global Instance RSym_open_func : RSym (@open_func typ _ _) :=
-	  @RSym_OpenFunc _ _ _ RType_typ _ _ _ _ _ _.
-
+(*
+  Global Instance RSym_open_func : RSym (@subst_func typ) :=
+	  @RSym_SubstFunc _ _ _ _ _ _ _ RType_typ _ _ _ _ _ _.
+*)
   Global Existing Instance RSym_sum.
   Global Existing Instance RSymOk_sum.
 
-  Global Instance RSym_func : RSym func.
-    repeat (apply RSym_sum; [|apply _]).
-    apply (RSym_func java_env).
-  Defined.
-  
-  Global Instance RSymOk_func : RSymOk RSym_func.
+  Definition RSym_sub_func (p : positive) :
+    RSym (match pmap_lookup' func_map p with | Some T => T | None => Empty_set end).
   Proof.
-    repeat (apply RSymOk_sum); try apply _.
-  Qed.
+    destruct p; simpl; [| | apply _].
+    destruct p; simpl; [| | apply _].
+    destruct p; simpl; [| | apply _].
+    induction p; simpl; intuition; apply RSym_Empty_set.
+    destruct p; simpl; [| | apply _].
+    induction p; simpl; intuition; apply RSym_Empty_set.
+    induction p; simpl; intuition; apply RSym_Empty_set.
+    destruct p; simpl; [| | apply _].
+    induction p; simpl; intuition; apply RSym_Empty_set.
+    destruct p; simpl; [| | apply _].
+    induction p; simpl; intuition; apply RSym_Empty_set.
+    induction p; simpl; intuition; apply RSym_Empty_set.
+    destruct p; simpl; [| | apply RSym_func; apply fs].
+    destruct p; simpl; [| | apply RSym_SubstFunc].
+    induction p; simpl; intuition; apply RSym_Empty_set.
+    destruct p; simpl; [| | apply _].
+    induction p; simpl; intuition; apply RSym_Empty_set.
+    induction p; simpl; intuition; apply RSym_Empty_set.
+    destruct p; simpl; [| | apply _].
+    induction p; simpl; intuition; apply RSym_Empty_set.
+    destruct p; simpl; [| | apply _].
+    induction p; simpl; intuition; apply RSym_Empty_set.
+    induction p; simpl; intuition; apply RSym_Empty_set.
+  Defined.
+Print RSymOk.
+Instance RSymOk_Empty_set : RSymOk RSym_Empty_set := {
+  sym_eqbOk a b :=
+    match a return (match sym_eqb a b with 
+                    | Some true => a = b 
+                    | Some false => a <> b
+                    | None => True
+                    end) with
+      end
+    
+}.
+
+  Lemma RSymOk_sub_func (p : positive) : RSymOk (RSym_sub_func p).
+  Proof.
+    destruct p; simpl; [| | apply _].
+    destruct p; simpl; [| | apply _].
+    destruct p; simpl; [| | apply _].
+    induction p; simpl; intuition; apply RSymOk_Empty_set.
+    destruct p; simpl; [| | apply _].
+    induction p; simpl; intuition; apply RSymOk_Empty_set.
+    induction p; simpl; intuition; apply RSymOk_Empty_set.
+    destruct p; simpl; [| | apply _].
+    induction p; simpl; intuition; apply RSymOk_Empty_set.
+    destruct p; simpl; [| | apply _].
+    induction p; simpl; intuition; apply RSymOk_Empty_set.
+    induction p; simpl; intuition; apply RSymOk_Empty_set.
+    destruct p; simpl; [| | apply _].
+    destruct p; simpl; [| | apply _].
+    induction p; simpl; intuition; apply RSymOk_Empty_set.
+    destruct p; simpl; [| | apply _].
+    induction p; simpl; intuition; apply RSymOk_Empty_set.
+    induction p; simpl; intuition; apply RSymOk_Empty_set.
+    destruct p; simpl; [| | apply _].
+    induction p; simpl; intuition; apply RSymOk_Empty_set.
+    destruct p; simpl; [| | apply _].
+    induction p; simpl; intuition; apply RSymOk_Empty_set.
+    induction p; simpl; intuition; apply RSymOk_Empty_set.
+  Defined.
+
+  Global Instance RSym_func : RSym func := RSymOneOf func_map RSym_sub_func.
+  
+  Global Instance RSymOk_func : RSymOk RSym_func := RSymOk_OneOf func_map RSym_sub_func RSymOk_sub_func.
 
   Global Instance Expr_expr : ExprI.Expr _ (expr typ func) := @Expr_expr typ func _ _ _.
   Global Instance Expr_ok : @ExprI.ExprOk typ RType_typ (expr typ func) Expr_expr := @ExprOk_expr _ _ _ _ _ _ _ _.
@@ -340,13 +469,17 @@ Check RSym.
     admit.
   Qed.
 *)
+(*
   Lemma evalDexpr_wt (e : dexpr) : 
 	  typeof_expr nil nil (evalDExpr e) = Some tyExpr.
-  Proof.
+  Proof. 
+    (* Not true anymore, need to fix *)
+
     induction e.
+    + simpl. admit.
     + simpl; reflexivity.
-    + simpl; reflexivity.
-    + simpl; rewrite IHe1, IHe2; reflexivity.
+    + simpl. rewrite IHe1.
+simpl; rewrite IHe1, IHe2; reflexivity.
     + simpl; rewrite IHe1, IHe2; reflexivity.
     + simpl; rewrite IHe1, IHe2; reflexivity.
     + simpl; rewrite IHe1, IHe2; reflexivity.
@@ -355,7 +488,8 @@ Check RSym.
     + simpl; rewrite IHe1, IHe2; reflexivity.
     + simpl; rewrite IHe1, IHe2; reflexivity.
   Qed.
-
+*)
+(*
   Definition is_pure (e : expr typ func) : bool :=
 	match e with
 	  | App f P => match embedS f with
@@ -371,20 +505,21 @@ Check RSym.
  		  | _ => false
  		end
    end.
-
+*)
   Definition mkPointstoVar x f e : expr typ func :=
      mkAp tyVal tyAsn 
           (mkAp tyString (tyArr tyVal tyAsn)
                 (mkAp tyVal (tyArr tyString (tyArr tyVal tyAsn))
-                      (mkConst (tyArr tyVal (tyArr tyString (tyArr tyVal tyAsn))) 
+                      (mkPure (tyArr tyVal (tyArr tyString (tyArr tyVal tyAsn))) 
                                fPointsto)
-                      (App fStackGet (mkString x)))
-                (mkConst tyString (mkString f)))
+                      (App (Inj fStackGet) (mkString x)))
+                (mkPure tyString (mkString f)))
           e.
-
+(*
   Definition test_lemma :=
     @lemmaD typ (expr typ func) RType_typ Expr_expr (expr typ func)
             (fun tus tvs e => exprD' tus tvs tyProp e)
             _
             nil nil.
+*)
 End JavaFunc.
